CTL

src/CTL.lean
@@ -20,13 +20,14 @@ open state_formula
 open path_formula
 
 local notation  `∼` Φ := neg Φ
-local notation Φ `and` Ψ := conj Φ Ψ
+local notation Φ `&` Ψ := conj Φ Ψ
 local notation `●` Φ := next Φ
 local notation Φ `𝒰` Ψ := until Φ Ψ
 
 structure TS :=
 (S : Type)
-(H : decidable_eq S)
+(H1 : inhabited S)
+(H2 : decidable_eq S)
 (Act : Type)
 (TR : set (S × Act × S))
 (L  : S → set AP)
@@ -36,23 +37,20 @@ def Post_of  {M : TS AP} (s : M.S) (α : M.Act) : set (M.S) := {s' | (s,α,s') �
 def Post {M : TS AP} (s : M.S) : set (M.S) :=
 ⋃ α : M.Act, Post_of _ s α
 
-def fin_path {AP : Type} (M : TS AP) : Type := 
-{l : list M.S // ∀ i : ℕ, }
 
 def path {AP : Type} (M : TS AP) : Type := 
 {s : stream M.S // ∀ i : ℕ, s (i + 1) ∈ Post _ (s i)}
 
-def first {M : TS AP} (π : path  M) : M.S := π.val 0
 
 def paths {AP : Type}
 {M : TS AP} (s : M.S) : set (path M) :=
-(λ π, s = (first _ π))
+(λ π, s =  π.val.head)
 
 mutual def state_sat, path_sat {M : TS AP}
 with state_sat : state_formula AP → M.S → Prop
 | T := λ _, true
 | (atom a) := λ s, a ∈ M.L s
-| (Φ and Ψ) := λ s, state_sat Φ s ∧ state_sat Ψ s
+| (Φ & Ψ) := λ s, state_sat Φ s ∧ state_sat Ψ s
 | (∼ Φ) := λ s, ¬ (state_sat Φ s)
 | (E φ) := λ s, ∃ π : path M, π ∈ paths s ∧ path_sat φ π
 | (A φ) := λ s, ∀ π : path M, π ∈ paths s → path_sat φ π
@@ -69,9 +67,9 @@ def potentially (φ : state_formula AP) : state_formula AP :=
 E(T 𝒰 φ)
 notation `E◆` φ := potentially _ φ 
 
-def inevitable (φ : state_formula AP) : state_formula AP := 
+def inevitably (φ : state_formula AP) : state_formula AP := 
 A(T 𝒰 φ)
-notation `A◆` φ := inevitable _ φ 
+notation `A◆` φ := inevitably _ φ 
 
 
 def potentially_always (φ : state_formula AP) : state_formula AP := 
@@ -85,16 +83,122 @@ notation `A◾` φ := invariantly _ φ
 
 namespace sat 
 
-def potentially {AP : Type} {M : TS AP} (φ : state_formula AP) (s : M.S): 
-(s ⊨ₛ φ) ↔ ∃ π ∈ paths s, ∃ j:ℕ, (subtype.val π j) ⊨ₛ φ := 
+def potentially {AP : Type} {M : TS AP} 
+(φ : state_formula AP) (s : M.S): 
+(s ⊨ₛ E◆φ) ↔ ∃ π ∈ paths s, ∃ j:ℕ, (subtype.val π j) ⊨ₛ φ := 
 begin 
+    rw [potentially,state_sat,path_sat], dsimp only,
     split,
-    intro s,
-    
+    { rintro ⟨π,H,j,Hj1,Hj2⟩,
+      use π, exact ⟨H, ⟨j,Hj1⟩⟩},
+    { rintro ⟨π,H1,j,H2⟩,
+      use π, 
+      split, {exact H1}, 
+     {use j, split, exact H2, intros, trivial}}
+end 
+
+def inevitably {AP : Type} {M : TS AP} 
+(φ : state_formula AP) (s : M.S) : 
+(s ⊨ₛ A◆φ) ↔ ∀ π ∈ paths s, ∃ j : ℕ, (subtype.val π j) ⊨ₛ φ := 
+begin
+    rw [inevitably,state_sat,path_sat], dsimp only,
+    split,
+    { intros H1 π H2, replace H1 := H1 π H2,
+      cases H1 with j H1,
+      use j, exact H1.1},
+    { intros H1 π H2, replace H1 := H1 π H2,
+      cases H1 with j H1,
+      use j, split, {exact H1}, intros, trivial}  
+end  
+
+
+def potentially_always {AP : Type} {M : TS AP}
+(φ : state_formula AP) (s : M.S) : 
+(s ⊨ₛ E◾φ) ↔ (∃ π ∈ paths s, ∀ j : ℕ, (subtype.val π j) ⊨ₛ φ) := 
+begin 
+    rw potentially_always,
+    rw state_sat, dsimp only, 
+    rw [inevitably,state_sat],
+    simp,
+end 
+
+def invariantly {AP : Type} {M : TS AP}
+(φ : state_formula AP) (s : M.S) : 
+(s ⊨ₛ A◾φ) ↔ (∀ π ∈ paths s, ∀ j : ℕ, (subtype.val π j) ⊨ₛ φ) := 
+begin 
+    rw invariantly,
+    rw state_sat, dsimp only, 
+    rw [potentially,state_sat],
+    simp,
+end 
+
+end sat
+
+def sat_set {AP : Type} (M : TS AP) (φ : state_formula AP): set M.S := 
+{s | s ⊨ₛ φ}
+
+def equiv {AP : Type} (φ ψ: state_formula AP) : Prop :=  
+∀ M : TS AP, (sat_set M φ) = (sat_set M ψ)
+
+notation φ ` ≡ ` ψ := equiv φ ψ  
+
+lemma forall_next_dual (φ : state_formula AP) : 
+    (A●φ) ≡ (∼E(●∼φ)) := 
+begin
+    intros M, ext, repeat {rw sat_set}, simp,
+    rw [state_sat,path_sat],
+    repeat {rw state_sat}, rw [path_sat, state_sat],
+    simp
+end 
+
+lemma exists_next_dual (φ : state_formula AP) : 
+    (E●φ) ≡ (∼A(●∼φ)) := 
+begin
+    intros M, ext, repeat {rw sat_set}, simp,
+    rw [state_sat,path_sat],
+    repeat {rw state_sat}, rw [path_sat, state_sat],
+    simp
 end 
 
 
-end sat
+lemma potentially_dual (φ : state_formula AP) : 
+    (E◆φ) ≡ ∼(A◾∼φ) := 
+begin 
+    intros M, ext, repeat {rw sat_set}, simp,
+    rw [sat.potentially,state_sat],simp,
+    rw [sat.invariantly,state_sat],simp,
+end 
+
+lemma inevitably_dual (φ : state_formula AP) : 
+    (A◆φ) ≡ ∼(E◾∼φ) := 
+begin 
+    intros M, ext, repeat {rw sat_set}, simp,
+    rw [sat.inevitably,state_sat],simp,
+    rw [sat.potentially_always,state_sat],simp,
+end 
+
+
+lemma until_dual_fst (φ ψ : state_formula AP) : 
+    A(φ 𝒰 ψ) ≡ (∼E((∼ ψ) 𝒰 ((∼ φ) & (∼ ψ))) & ∼ E◾ (∼ ψ)) := 
+    begin
+        intros M, ext, repeat {rw sat_set}, simp,
+        repeat {rw [state_sat]},
+        repeat {rw [path_sat]}, simp,
+        split, {
+            intro H1,split,{
+                intros π H2 i H3,
+                repeat {rw state_sat at H3},
+                rw state_sat, simp at *,
+                replace H1 := H1 π H2,
+                cases H1 with j Hj,
+                sorry 
+            },{
+                sorry
+            }
+        },{sorry}
+    end 
+
+
 
 
 end CTL
